LeanPlayground/LC3/Encodable.lean
@@ -1,0 +1,324 @@
+import Std.Tactic.Basic
+
+import LeanPlayground.Data.Nat.Pairing
+
+/-!
+# Encoding data into numerals
+
+We define a type class `Encodable α ν` asserting that `α` is encoded into `ν`.
+More precisely, it has the following methods:
+
+- `Encodable.encode : α → ν`
+- `Encodable.decode : ν → α`
+- `Encodable.decode_encode : ∀ (a : α), decode (encode a) = a`
+
+## Remark
+
+The method `Encodable.decode` is a total function just for the simplicity.
+As a result, one cannot write instances for empty types such as `Fin 0` unless the encoded type `ν` is empty.
+One can of course define a version with a decoder as a partial function if necessary.
+-/
+
+-- Disable auto-binding of unbounded variables
+set_option autoImplicit false
+
+/-!
+### Preliminaries
+-/
+
+namespace Prod
+
+universe u₁ u₂ v₁ v₂
+
+theorem map_fst {α₁ : Type u₁} {α₂ : Type u₂} {β₁ : Type v₁} {β₂ : Type v₂} (f : α₁ → α₂) (g : β₁ → β₂) (p : α₁ × β₁) : (p.map f g).fst = f p.fst :=
+  rfl
+
+theorem map_snd {α₁ : Type u₁} {α₂ : Type u₂} {β₁ : Type v₁} {β₂ : Type v₂} (f : α₁ → α₂) (g : β₁ → β₂) (p : α₁ × β₁) : (p.map f g).snd = g p.snd :=
+  rfl
+
+
+end Prod
+
+namespace Nat
+
+protected class Positive (n : Nat) : Prop where
+  positive : n > 0
+
+instance succ_positive (n : Nat) : Nat.Positive (n+1) where
+  positive := n.succ_pos
+
+namespace Positive
+
+protected theorem ne_zero {n : Nat} [Nat.Positive n] : n ≠ 0 :=
+  Nat.ne_of_gt Positive.positive
+
+end Positive
+
+end Nat
+
+namespace Int
+
+theorem negSucc_lt_ofNat (m n : Nat) : -[m+1] < ↑(n : Nat) := by
+  show (Int.ofNat n - (-[m+1] + 1)).NonNeg
+  conv => arg 1; equals .ofNat (n+m) =>
+    rewrite [Int.negSucc_eq, Int.neg_add, Int.neg_add_cancel_right, Int.sub_neg]
+    rfl
+  exact .mk (n+m)
+
+theorem toNat_lt' {a : Int} {n : Nat} (h : n > 0) : a.toNat < n ↔ a < ↑(n : Nat) := by
+  match a with
+  | .ofNat k => simp
+  | -[k+1] =>
+    simp only [Int.toNat, iff_true_left h]
+    exact negSucc_lt_ofNat k n
+
+--theorem emod_ofNat_lt (a : Int) {n : Nat} (h : n > 0) : a % ↑n < n := by
+  --sorry
+
+@[inline]
+protected def pair (a b : Int) : Int :=
+  let rec tonat (a : Int) : Nat :=
+    match a with
+    | .ofNat n => 2*n
+    | -[n+1]   => 2*n+1
+  match a with
+  | .ofNat m => .ofNat <| Nat.pair m (tonat b)
+  | -[m+1]   => -[Nat.pair m (tonat b)+1]
+
+protected def unpair (a : Int) : Int × Int :=
+  let rec fromnat (n : Nat) : Int :=
+    if n % 2 = 0 then .ofNat (n/2) else -[n/2+1]
+  match a with
+  | .ofNat n => Prod.map ofNat fromnat <| Nat.unpair n
+  | -[n+1] => Prod.map negSucc fromnat <| Nat.unpair n
+
+theorem unpair_pair (a b : Int) : Int.unpair (Int.pair a b) = (a,b) := by
+  cases a <;> cases b <;> rename_i m n
+    <;> all_goals refine Prod.ext ?_ ?_
+    <;> dsimp [Int.pair, pair.tonat, Int.unpair]
+    <;> simp only [Prod.map_fst, Prod.map_snd, Nat.unpair_pair]
+    <;> try rfl
+  all_goals
+    unfold unpair.fromnat
+    simp only [Nat.mul_mod_right 2 n, Nat.mul_add_mod 2 n 1, if_true, if_false]
+    simp only [Nat.mul_div_right n Nat.two_pos, Nat.mul_add_div Nat.two_pos]
+    rfl
+
+end Int
+
+
+/-!
+### Definition
+-/
+
+namespace LC3
+
+universe u v
+
+class Encodable (α : Type u) (ν : Type v) where
+  encode : α → ν
+  decode : ν → α
+  decode_encode : ∀ (a : α), decode (encode a) = a
+
+namespace Encodable
+
+/-!
+### Basic declarations
+-/
+
+/-- Every type can be trivially encoded into itself with `id` -/
+protected instance (priority:=high) instId (α : Type u) : Encodable α α where
+  encode := id
+  decode := id
+  decode_encode _ := rfl
+
+
+/-!
+### Encoding into `Nat`
+-/
+
+section Nat
+
+variable {α : Type u} {β : Type v} [Encodable α Nat] [Encodable β Nat]
+
+protected instance instFinNat (n : Nat) [Nat.Positive n] : Encodable (Fin n) Nat where
+  encode := Fin.val
+  decode k := ⟨k % n, k.mod_lt Nat.Positive.positive⟩
+  decode_encode i := Fin.eq_of_val_eq <| i.1.mod_eq_of_lt i.2
+
+protected instance instFinProdNat (n : Nat) [Nat.Positive n] : Encodable (Fin n × α) Nat where
+  encode x := x.1.1 + n * encode x.2
+  decode k := (⟨k % n, k.mod_lt Nat.Positive.positive⟩, decode (k / n))
+  decode_encode x := by
+    refine Prod.ext (Fin.eq_of_val_eq ?_) ?_
+    . show (x.1.1 + n * encode x.2) % n = x.1.1
+      rewrite [Nat.add_mul_mod_self_left]
+      exact x.1.1.mod_eq_of_lt x.1.2
+    . show decode ((x.1.1 + n * encode x.2) / n) = x.2
+      rewrite [Nat.add_mul_div_left x.1.1 _ Nat.Positive.positive]
+      rewrite [Nat.div_eq_of_lt x.1.2, Nat.zero_add]
+      exact decode_encode x.2
+
+attribute [irreducible] Encodable.decode in
+protected instance instBoolProdNat : Encodable (Bool × α) Nat where
+  encode x := encode (Fin.mk (n:=2) x.1.toNat x.fst.toNat_lt, x.2)
+  decode p := Prod.map (· == 1) id <| (decode p : Fin 2 × α)
+  decode_encode x := by
+    rcases x with ⟨b, a⟩
+    simp only [Prod.map, decode_encode, id]
+    refine Prod.ext ?_ rfl
+    simp only
+    cases b <;> dsimp [Bool.toNat] <;> decide
+
+protected instance instSumNat : Encodable (α ⊕ β) Nat where
+  encode p :=
+    match p with
+    | .inl a => 2 * encode a
+    | .inr b => 1 + 2 * encode b
+  decode k :=
+    if k % 2 = 0 then
+      .inl <| decode (k/2)
+    else
+      .inr <| decode (k/2)
+  decode_encode p := by
+    match p with
+    | .inl a =>
+      simp only [Nat.mul_mod_right, ite_true, Nat.mul_div_right _ Nat.two_pos]
+      exact congrArg Sum.inl <| decode_encode a
+    | .inr b =>
+      simp only [Nat.add_mul_mod_self_left, ite_false, Nat.add_mul_div_left 1 _ Nat.two_pos, Nat.div_eq_of_lt (Nat.succ_lt_succ Nat.one_pos), Nat.zero_add]
+      exact congrArg Sum.inr <| decode_encode b
+
+open Int in
+protected instance instIntNat : Encodable Int Nat where
+  encode k :=
+    match k with
+    | .ofNat n => 2 * n
+    | -[n+1] => 1 + 2 * n
+  decode n :=
+    if n % 2 = 0 then
+      .ofNat (n/2)
+    else
+      -[n/2+1]
+  decode_encode k := by
+    match k with
+    | .ofNat n =>
+      simp only [Nat.mul_mod_right, ite_true, Nat.mul_div_right _ Nat.two_pos]
+    | -[n+1] =>
+      simp only [Nat.add_mul_mod_self_left, ite_false]
+      rewrite [Nat.add_mul_div_left 1 _ Nat.two_pos, Nat.add_comm]
+      rfl
+
+protected instance instCharNat : Encodable Char Nat where
+  encode c := c.toNat
+  decode n := Char.ofNat n
+  decode_encode c := by
+    rcases c with ⟨⟨c,hlt⟩, hvalid⟩
+    dsimp only [Char.ofNat, Char.toNat, Char.ofNatAux]
+    dsimp [UInt32.isValidChar, UInt32.toNat] at hvalid ⊢
+    simp only [Int.toNat_ofNat, dif_pos hvalid]
+
+protected instance (priority:=low) instProdNat : Encodable (α × β) Nat where
+  encode x := Nat.pair (encode x.1) (encode x.2)
+  decode n := Prod.map decode decode n.unpair
+  decode_encode x := by
+    simp only [Nat.unpair_pair]
+    simp only [Prod.map, decode_encode]
+
+end Nat
+
+
+/-!
+### Encoding into `Int`
+-/
+
+section Int
+
+variable {α : Type u} {β : Type v} [Encodable α Int] [Encodable β Int]
+
+protected instance (priority:=low+1) instOfNatInt (α : Type u) [Encodable α Nat] : Encodable α Int where
+  encode a := ↑(encode a : Nat)
+  decode k := decode k.toNat
+  decode_encode a := by
+    simp only [Int.toNat_ofNat]
+    exact decode_encode a
+
+attribute [irreducible] Encodable.decode in
+protected instance (priority:=high+1) instFinProdInt (n : Nat) [Nat.Positive n] : Encodable (Fin n × α) Int where
+  encode p := p.1.1 + n * encode p.2
+  decode k :=
+    have := by
+      refine Int.toNat_lt' Nat.Positive.positive |>.mpr ?_
+      refine Int.emod_lt_of_pos k ?_
+      exact Int.ofNat_pos.mpr Nat.Positive.positive
+    (⟨Int.toNat (k % n), this⟩, decode (k / n))
+  decode_encode x :=
+    match x with
+    | (i,a) => by
+      refine Prod.ext (Fin.eq_of_val_eq ?_) ?_
+      . show Int.toNat ((i.val + n * (encode a : Int)) % n) = i.val
+        rewrite [Int.add_mul_emod_self_left i.val n _]
+        exact i.val.mod_eq_of_lt i.isLt
+      . show decode ((i.val + n * (encode a : Int)) / n) = a
+        have : ↑(n : Nat) ≠ (0 : Int) := by
+          intro h; rcases h with ⟨rfl⟩; nomatch i
+        rewrite [Int.mul_comm ↑n _, Int.add_mul_ediv_right _ _ this]
+        rewrite [← Int.ofNat_ediv, i.val.div_eq_of_lt i.isLt]
+        simp_arith
+        exact decode_encode a
+
+attribute [irreducible] Encodable.decode in
+protected instance instBoolProdInt : Encodable (Bool × α) Int where
+  encode x := encode (Fin.mk (n:=2) x.1.toNat x.fst.toNat_lt, x.2)
+  decode p := Prod.map (· == 1) id <| (decode p : Fin 2 × α)
+  decode_encode x := by
+    rcases x with ⟨b, a⟩
+    simp only [Prod.map, decode_encode, id]
+    refine Prod.ext ?_ rfl
+    simp only
+    cases b <;> dsimp [Bool.toNat] <;> decide
+
+open Int in
+attribute [irreducible] Encodable.decode in
+protected instance (priority:=low+1) instProdInt : Encodable (α × β) Int where
+  encode x :=
+    match (encode x.1 : Int) with
+    | .ofNat n => .ofNat <| encode (n, (encode x.2 : Int))
+    | -[n+1] => -[encode (n, (encode x.2 : Int))+1]
+  decode k :=
+    match k with
+    | .ofNat n => Prod.map (decode ∘ Int.ofNat) decode <| (decode n : Nat × Int)
+    | -[n+1] => Prod.map (decode ∘ Int.negSucc) decode <| (decode n : Nat × Int)
+  decode_encode x := by
+    rcases x with ⟨a,b⟩
+    simp only
+    cases h : (encode a : Int)
+    all_goals
+      simp only [decode_encode, Prod.map, Function.comp]
+      rw [← h, decode_encode]
+
+end Int
+
+
+/-
+# Test codes
+-/
+/-- info: 267 -/
+#guard_msgs in
+#eval (encode ((3 : Fin 8), (1 : Fin 8), (4 : Nat)) : Int)
+
+/-- info: (3, 1, 4) -/
+#guard_msgs in
+#eval (decode 267 : Fin 8 × Fin 8 × Nat)
+
+/-- info: -83 -/
+#guard_msgs in
+#eval (encode (true, -42) : Int)
+
+/-- info: (true, -42) -/
+#guard_msgs in
+#eval (decode (-83) : Bool × Int)
+
+end Encodable
+
+end LC3
