LeanPlayground/LC3/ISA.lean
@@ -1,0 +1,279 @@
+import LeanPlayground.LC3.Encodable
+
+/-!
+# ISA of LC-3 architecture
+
+We define the ***ISA*** (*I*nstruction *S*et *A*rchitecture) of LC-3 architecture.
+The original resource of the architecture is found in *Introduction to Computing Systems* by Yale Patt and Sanjay Patel.
+-/
+
+-- Disable auto-binding of unbounded variables
+set_option autoImplicit false
+
+namespace LC3
+
+/-!
+### The second operand of ALU
+
+In the LC-3 architecture, every binary operation (i.e. *ADD*, *AND*, and *XOR* in ALU instruction can take a register and an immediate value as the second operand.
+-/
+
+/-- The second operand of binary operations (i.e. *ADD*, *AND*, and *XOR*) is either a register or an immediate value. -/
+inductive RHSVal where
+| reg : Fin 8 → RHSVal
+| imm : Int → RHSVal
+deriving DecidableEq, Repr
+
+namespace RHSVal
+
+open Encodable in
+instance : Encodable RHSVal Int where
+  encode x :=
+    match x with
+    | .reg i => encode (Sum.inl (β:=Int) i)
+    | .imm n => encode (Sum.inr (α:=Fin 8) n)
+  decode n :=
+    match (decode n : Fin 8 ⊕ Int) with
+    | .inl i => .reg i
+    | .inr n => .imm n
+  decode_encode x := by
+    cases x with
+    | reg i => simp only [decode_encode]
+    | imm n => simp only [decode_encode]
+
+end RHSVal
+
+
+/-!
+### Definition of ISA
+-/
+
+/--
+The ISA (Instruction Set Architecture) of *LC-3* architecture.
+It assumes the following registers in addition to the main registers:
+- ***PC*** (*P*rogram *C*ounter) containing the address in the memory of the next instruction to be executed.
+- ***PSR*** (*P*rocessor *S*tatus *R*egister) maintaining
+  - `n`-flag stands for the last ALU / load operation results in negative;
+  - `z`-flag stands for the last ALU / load operation results in zero;
+  - `p`-flag stands for the last ALU / load operation results in positive;
+  - the execution mode: either `.user` or `.privilege`;
+  - the execution priority level.
+- ***Saved_SP***
+Two ranges in the main memory are used for *stacks*; one for the *User Stack* and the other for the *Supervisor Stack*.
+The stack pointers for them are called ***USP*** (User Stack Pointer) and ***SSP*** (Supervisor Stack Pointer) respectively .
+  - If `PSR.mode = .user`, then ***USP*** is maintained by one of the registers (e.g. the 6-th in the original LC-3) while ***SSP*** is stored in ***Saved_SP***.
+  - If `PSR.mode = .privilege`, then the other way.
+-/
+inductive ISA where
+/--
+*Conditional Branch* instruction: `br n z p imm` is the conditional jump to `PC + imm` based on the `n`, `z`, and `p` flags.
+It causes `PC ← PC + imm` in either of the following case:
+- `n = true` and the `n`-flag is set;
+- `z = true` and the `z`-flag is set;
+- `p = true` and the `p`-flag is set.
+-/
+| br (n p z : Bool) (imm : Int) : ISA
+/--
+*Addition* instruction: `add dr sr1 rhs` causes `dr ← sr1 + rhs`, where `rhs` is either a register `RHSVal.reg sr2` or an immediate value `RHSVal.imm imm`.
+The `n`-, `z`-, and `p`-flags should be set properly afterwards.
+-/
+| add (dr sr1 : Fin 8) (rhs : RHSVal) : ISA
+/--
+*Load* instruction: `ld dr imm` causes `dr ← mem[PC + imm]`.
+If `PSR.mode = .user`, then the instruction gives rise to an ACV exception in the case `PC + imm` lies in the privileged range.
+The `n`-, `z`-, and `p`-flags should be set properly afterwards.
+-/
+| ld (dr : Fin 8) (imm : Int) : ISA
+/--
+*Store* instruction: `st sr imm` causes `mem[PC + imm] ← sr`.
+If `PSR.mode = .user`, then the instruction gives rise to an ACV exception in the case `PC + imm` lies in the privileged range.
+-/
+| st (sr : Fin 8) (imm : Int) : ISA
+/--
+*Jump to Subroutine* instruction: `jsr dr (.reg sr)` is equivalent to the following pseudo-code:
+```
+AUX ← PC;
+PC ← sr;
+dr ← AUX;
+```
+`jsr dr (.imm imm)` causes `dr ← PC; PC ← PC + imm`.
+
+* Remark
+In the original LC-3, the *JSR* instruction stands for `jsr 7 (.reg sr)` while *JSRR* for `jsr 7 (.imm imm)`.
+For both instructions, one cannot specify the destination register since the 7-th register is distinguished to interact with `PC`.
+See also the remark in `LC3.ISA.jmp`.
+-/
+| jsr (dr : Fin 8) : RHSVal → ISA
+/--
+*Bitwise Logical AND* instruction: `and dr sr1 rhs` causes `dr ← sr1 &&& rhs`, where `rhs` is either a register `RHSVal.reg sr2` or an immediate value `RHSVal.imm imm`.
+The `n`-, `z`-, and `p`-flgas are set properly afterwards.
+-/
+| and (dr sr1 : Fin 8) (rhs : RHSVal) : ISA
+/--
+*Load Base+offset* instruction: `ldr dr sr imm` causes `dr ← mem[sr + imm]`.
+If `PSR.mode = .user`, then the instruction gives rise to an ACV exception in the case `sr + imm` lies in the privileged range.
+The `n`-, `z`-, and `p`-flags are set properly afterwards based on the loaded value.
+-/
+| ldr (dr sr : Fin 8) (imm : Int) : ISA
+/--
+*Store Base+offset* instruction: `str sr dr imm` causes `mem[dr + imm] ← sr`.
+If `PSR.mode = .user`, then the instruction gives rise to an ACV exception in the case `dr + imm` lies in the privileged range.
+-/
+| str (sr dr : Fin 8) (imm : Int) : ISA
+/--
+*Return from Trap or Interrupt* instruction: `rti spr` is equivalent to the following pseudo-code:
+```
+if PSR.mode == .user then
+  throw PRIVILEGE_MODE_EXCEPTION;
+
+PC ← mem[spr];
+spr ← spr + 1;
+PSR ← mem[spr];
+AUX ← spr + 1;
+if PSR.mode == .user then
+  spr ← Saved_SP;
+  Saved_SP ← AUX;
+else
+  spr ← AUX;
+```
+The instruction assumes that the `spr` is the register containing the supervisor stack pointer with the following stack structure:
+```
+──────────────
+|   . . .    |
+──────────────
+| Caller PC  | <- spr
+──────────────
+| Caller PSR |
+──────────────
+|   . . .    |
+──────────────
+| Stack Base |
+──────────────
+```
+-/
+| rti (spr : Fin 8) : ISA
+/--
+*Bitwise Logical XOR* instruction: `not dr sr1 rhs` causes `dr ← sr1 ^^^ rhs`, where `rhs` is either a register `RHSVal.reg sr2` or an immediate value `RHSVal.imm imm`.
+The `n`-, `z`-, and `p`-flags are set property aftterwards.
+
+* Remark
+In the original LC-3 has *NOT* instruction instead of the XOR-operation.
+In fact, one can think of it as `xor dr sr (.imm (-1))`.
+-/
+| xor (dr sr1 : Fin 8) (rhs : RHSVal) : ISA
+/--
+*Load Indirect* instruction: `ldi dr imm` causes `dr ← mem[mem[PC + imm]]`.
+If `PSR.mode = .privilege`, then the instruction gives rise to an ACV exception in the case either of `PC + imm` or `mem[PC + imm]` lies in the privileged range.
+The `n`-, `z`-, and `p`-flags should be set properly afterwards.
+-/
+| ldi (dr : Fin 8) (imm : Int) : ISA
+/--
+*Store Indirect* instruction: `sti sr imm` causes `mem[mem[PC + imm]] ← sr`.
+If `PSR.mode = .privilege`, then the instruction gives rise to an ACV exception in the case either of `PC + imm` or `mem[PC + imm]` lies in the privileged range.
+-/
+| sti (sr : Fin 8) (imm : Int) : ISA
+/--
+*Jump* instruction: `jmp sr` causes `PC ← sr`.
+
+* Remark
+ In the original LC-3, `jmp 7` is especially denoted by *RET* and called *Return from Subroutine* instruction since the 7-th register is distinguished to interact with `PC`.
+ See also the remark in `LC3.ISA.jsr`.
+-/
+| jmp (sr : Fin 8) : ISA
+/--
+The instruction for the *reserved* opcode (`0b1101`).
+-/
+| reserved (n : Int) : ISA
+/--
+*Load Effective Address* instruction: `lea dr imm` causes `dr ← PC + imm`.
+-/
+| lea (dr : Fin 8) (imm : Int) : ISA
+/--
+*System Call* instruction: `trap spr tv` is equivalent to the following pseudo-code:
+```
+AUX ← PSR;
+if PSR.mode = .user
+  swap (Saved_SP, spr);
+  PSR.mode ← .privilege;
+spr ← spr - 1;
+mem[spr] ← AUX;
+spr ← spr - 1;
+mem[spr] ← PC;
+PC ← mem[tv];
+```
+The memory range where `tv` can point to is called **Trap Vector Table**, and the actual execution codes stored there are implementation-defined.
+-/
+| trap (spr : Fin 8) (tv : Int) : ISA
+deriving DecidableEq, Repr
+
+namespace ISA
+
+open Encodable in
+instance : Encodable ISA Int where
+  encode instr :=
+    match instr with
+    | br p z n imm => encode ((0x0 : Fin 16), (encode (p, z, n, imm) : Int))
+    | add dr sr1 rhs => encode ((0x1 : Fin 16), (encode (dr, sr1, rhs) : Int))
+    | ld dr imm => encode ((0x2 : Fin 16), (encode (dr, imm) : Int))
+    | st sr imm => encode ((0x3 : Fin 16), (encode (sr, imm) : Int))
+    | jsr dr rhs => encode ((0x4 : Fin 16), (encode (dr, rhs) : Int))
+    | and dr sp1 rhs => encode ((0x5 : Fin 16), (encode (dr, sp1, rhs) : Int))
+    | ldr dr sr imm => encode ((0x6 : Fin 16), (encode (dr, sr, imm) : Int))
+    | str sr dr imm => encode ((0x7 : Fin 16), (encode (sr, dr, imm) : Int))
+    | rti spr => encode ((0x8 : Fin 16), (encode spr : Int))
+    | xor dr sr1 rhs => encode ((0x9 : Fin 16), (encode (dr, sr1, rhs) : Int))
+    | ldi dr imm => encode ((0xA : Fin 16), (encode (dr, imm) : Int))
+    | sti sr imm => encode ((0xB : Fin 16), (encode (sr, imm) : Int))
+    | jmp sr => encode ((0xC : Fin 16), (encode sr : Int))
+    | reserved n => encode ((0xD : Fin 16), (encode n : Int))
+    | lea dr imm => encode ((0xE : Fin 16), (encode (dr, imm) : Int))
+    | trap spr tv => encode ((0xF : Fin 16), (encode (spr, tv) : Int))
+  decode n :=
+    match decode (α:=Fin 16 × Int) n with
+    | (0x0, n) => let (p,z,n,imm) := decode n; .br p z n imm
+    | (0x1, n) => let (dr, sr1, rhs) := decode n; .add dr sr1 rhs
+    | (0x2, n) => let (dr, imm) := decode n; .ld dr imm
+    | (0x3, n) => let (sr, imm) := decode n; .st sr imm
+    | (0x4, n) => let (dr, rhs) := decode n; .jsr dr rhs
+    | (0x5, n) => let (dr, sr1, rhs) := decode n; .and dr sr1 rhs
+    | (0x6, n) => let (dr, sr, imm) := decode n; .ldr dr sr imm
+    | (0x7, n) => let (sr, dr, imm) := decode n; .str sr dr imm
+    | (0x8, n) => .rti <| decode n
+    | (0x9, n) => let (dr, s1, rhs) := decode n; .xor dr s1 rhs
+    | (0xA, n) => let (dr, imm) := decode n; .ldi dr imm
+    | (0xB, n) => let (sr, imm) := decode n; .sti sr imm
+    | (0xC, n) => .jmp <| decode n
+    | (0xD, n) => .reserved <| decode n
+    | (0xE, n) => let (dr, imm) := decode n; .lea dr imm
+    | (0xF, n) => let (spr,tv) := decode n; .trap spr tv
+    | (⟨_+16, h⟩, _) =>
+      have := Nat.lt_of_add_lt_add_right h
+      nomatch this
+  decode_encode instr := by
+    cases instr <;> simp only [decode_encode]
+
+/--
+*DO NOTHING* instruction.
+It is implemented as `br false false false 0`.
+Note that encoding this instruction into `Int` results in `0`; see `LC3.ISA.encode_none`.
+-/
+def none : ISA :=
+  .br false false false 0
+
+open Encodable in
+theorem encode_none : (encode ISA.none : Int) = 0 := by
+  decide
+
+/--
+*Bitwise Complement* instruction: `not dr sr` causes `dr ← ~~~sr`.
+
+* Remark
+Although the original LC-3 ISA has *NOT* as its 16 instructions, our version define it as a special case *XOR* as `not dr sr := xor dr sr (.imm (-1))`.
+-/
+def not (dr sr : Fin 8) : ISA :=
+  .xor dr sr (.imm (-1))
+
+end ISA
+
+
+end LC3
