LeanPlayground/LC3/Machine.lean
@@ -1,0 +1,391 @@
+import Std.Data.HashMap
+
+import LeanPlayground.Data.Int.Bit
+import LeanPlayground.LC3.Encodable
+import LeanPlayground.LC3.ISA
+
+/-!
+# A model of a machine for LC-3 ISA
+-/
+
+-- Disable auto-binding of unbounded variables
+set_option autoImplicit false
+
+namespace LC3
+
+/-!
+### Processor Status
+-/
+
+inductive ExecMode where
+| user
+| privilege
+deriving DecidableEq, Repr
+
+instance : Encodable ExecMode (Fin 2) where
+  encode x := match x with | .user => 0 | .privilege => 1
+  decode n := match n with | 0 => .user | 1 => .privilege
+  decode_encode x := by cases x <;> rfl
+
+structure ProcessorStatus where
+  (n z p : Bool)
+  (prio : Nat)
+  (mode : ExecMode)
+deriving DecidableEq, Repr
+
+open Encodable in
+instance : Encodable ProcessorStatus Int where
+  encode ps :=
+    encode (cond ps.n (1 : Fin 2) 0, cond ps.z (1 : Fin 2) 0, cond ps.p (1 : Fin 2) 0, (encode ps.mode : Fin 2), ps.prio)
+  decode n :=
+    let (n, z, p, mode, prio) : Fin 2 × Fin 2 × Fin 2 × Fin 2 × Nat :=
+      decode n
+    {
+      n := n == 1
+      z := z == 1
+      p := p == 1
+      mode := decode mode
+      prio := prio
+    }
+  decode_encode ps := by
+    simp only [decode_encode]
+    rcases ps with ⟨n,z,p,prio,mode⟩
+    cases n <;> cases z <;> cases p <;> rfl
+
+/-!
+### Memory addressing
+-/
+
+inductive Address where
+| trapvec (n : Int) : Address
+| privMem (n : Int) : Address
+| privStack (n : Int) : Address
+| userMem (n : Int) : Address
+| userStack (n : Int) : Address
+| device (i : Nat) (n : Int) : Address
+deriving DecidableEq, Repr, Hashable
+
+namespace Address
+
+open Encodable in
+instance : Encodable Address Int where
+  encode addr :=
+    match addr with
+    | .trapvec n => encode ((0 : Fin 6), n)
+    | .privMem n => encode ((1 : Fin 6), n)
+    | .privStack n => encode ((2 : Fin 6), n)
+    | .userMem n => encode ((3 : Fin 6), n)
+    | .userStack n => encode ((4 : Fin 6), n)
+    | .device i n => encode ((5 : Fin 6), (encode (i, n) : Int))
+  decode n :=
+    match (decode n : Fin 6 × Int) with
+    | (0, n) => .trapvec n
+    | (1, n) => .privMem n
+    | (2, n) => .privStack n
+    | (3, n) => .userMem n
+    | (4, n) => .userStack n
+    | (5, n) => let (i,n) := (decode n : Nat × Int); .device i n
+  decode_encode addr := by
+    cases addr <;> simp only [decode_encode]
+
+@[inline]
+def isUser (addr : @& Address) : Bool :=
+  match addr with
+  | .trapvec _ | privMem _ | privStack _ => false
+  | .userMem _ | .userStack _ | .device _ _ => true
+
+@[inline]
+def isPrivilege (addr : @& Address) : Bool :=
+  match addr with
+  | .trapvec _ | privMem _ | privStack _ => true
+  | .userMem _ | .userStack _ | .device _ _ => false
+
+@[inline]
+def map (f : Int → Int) : Address → Address
+| .trapvec n => .trapvec <| f n
+| .privMem n => .privMem <| f n
+| .privStack n => .privStack <| f n
+| .userMem n => .userMem <| f n
+| .userStack n => .userStack <| f n
+| .device i n => .device i <| f n
+
+instance : HAdd Address Int Address where
+  hAdd addr n := addr.map (· + n)
+
+end Address
+
+
+/-!
+### Definition of the machine
+-/
+
+structure Machine where
+  /-- Processor Status Register -/
+  psr : ProcessorStatus
+  /-- Instruction Register -/
+  ir : ISA
+  /-- Program Counter -/
+  pc : Address
+  /-- Machine Address Register -/
+  mar : Address
+  /-- Machine Data Register -/
+  mdr : Int
+  /-- Registers -/
+  reg : Array Int
+  reg_size_eq : reg.size = 8
+  /-- Saved Stack pointer register -/
+  sspr : Address
+  /-- Memory space -/
+  mem : Std.HashMap Address Int
+
+namespace Machine
+
+def init : Machine where
+  psr := ⟨false, true, false, 0, .privilege⟩
+  ir := .br false false false 0
+  pc := .privMem 0
+  mar := .privMem 0
+  mdr := default
+  reg := Array.mkArray 8 default
+  reg_size_eq := rfl
+  sspr := .userStack 0
+  mem := ∅
+
+instance : Inhabited Machine :=
+  ⟨init⟩
+
+@[inline]
+def getReg (m : @& Machine) (i : Fin 8) : Int :=
+  m.reg[i.1]'(m.reg_size_eq.symm ▸ i.2)
+
+@[inline]
+def setReg (m : Machine) (i : Fin 8) (n : Int) : Machine :=
+  {m with
+    reg := m.reg.set (i.cast m.reg_size_eq.symm) n
+    reg_size_eq := by
+      simp only [Array.size_set]
+      exact m.reg_size_eq
+  }
+
+@[inline]
+def getMem (m : @& Machine) (addr : Address) : Int :=
+  m.mem[addr].getD default
+
+@[inline]
+def setMem (m : Machine) (addr : Address) (n : Int) : Machine :=
+  {m with
+    mem := m.mem.insert addr n
+  }
+
+/--
+Set the *Conditional Code* (i.e. `p`-, `z`-, and `n`-flags) properly depending on the given value.
+-/
+@[inline]
+def setCC (m : Machine) (x : Int) : Machine :=
+  {m with
+    psr := {m.psr with
+      p := decide (x > 0)
+      z := decide (x = 0)
+      n := decide (x < 0)
+    }
+  }
+
+
+/-!
+### The instruction cycle
+
+The instruction cycle consists of the following phases:
+1. FETCH
+2. DECODE
+3. EVALUATE ADDRESS
+4. FETCH OPERANDS
+5. EXECUTE
+6. STORE RESULT
+-/
+
+open Encodable in
+/--
+The ***FETCH*** phase in the instruction cycle.
+It goes as follows:
+```
+MAR ← PC;
+PC ← PC + 1;
+MDR ← mem[MAR];
+IR ← MDR;
+```
+-/
+def fetch (m : Machine) : Machine :=
+  let m := {m with mar := m.pc}
+  let m := {m with pc := m.pc + (1 : Int)}
+  let m := {m with mdr := m.getMem m.mar}
+  {m with ir := decode m.mdr}
+
+/--
+The ***DECODE*** phase in the instruction cycle.
+The phase examines `IR` to determine what the architecture is to do.
+Although it is an important phase for physical machines, we just skip it as implementing just a logical model.
+-/
+def decode (m : Machine) : Machine :=
+  m
+
+/--
+The ***EVALUATE ADDRESS*** phase in the instruction cycle.
+The phase computes `reg + offset` for those instructions who requires it.
+- *BR*, *LD*, *ST*, *JSR* (with offset value), *LDI*, *STI*: `PC + offset`
+- *LDR*: `sr + offset`
+- *STR*: `dr + offset`
+Note that the last two cases requires decoding the content of the register into `Address`.
+-/
+def evalAddress (m : Machine) : Machine :=
+  match m.ir with
+  | .br _ _ _ imm => {m with mar := m.pc + imm}
+  | .add .. => m
+  | .ld _ imm => {m with mar := m.pc + imm}
+  | .st _ imm => {m with mar := m.pc + imm}
+  | .jsr _ (.reg _) => m
+  | .jsr _ (.imm imm) => {m with mar := m.pc + imm}
+  | .and .. => m
+  | .ldr _ sr imm =>
+    {m with mar := (Encodable.decode (m.getReg sr) : Address) + imm}
+  | .str _ dr imm =>
+    {m with mar := (Encodable.decode (m.getReg dr) : Address) + imm}
+  | .rti _ => m
+  | .xor .. => m
+  | .ldi _ imm => {m with mar := m.pc + imm}
+  | .sti _ imm => {m with mar := m.pc + imm}
+  | .jmp _ => m
+  | .reserved _ => m
+  | .lea _ imm => {m with mar := m.pc + imm}
+  | .trap .. => m
+
+/--
+The ***FETCH OPERANDS*** phase in the instruction cycle.
+It is only needed for *LOAD XXX* instructions; i.e. *LD*, *LDR*, *LDI*.
+More precisely, the phase causes `MDR ← mem[MAR]` for *LD* and *LDR* while `MDR ← mem[mem[MAR]]` for *LDI*.
+The phase may give rise to the ACV exception if `m.psr.mode = .user` and if the memory location lies in the privileged range.
+-/
+def fetchOp (m : Machine) : Option Machine :=
+  match m.ir with
+  | .ld .. | .ldr .. =>
+    if m.psr.mode == .user && m.mar.isPrivilege then
+      .none
+    else
+      .some {m with mdr := m.getMem m.mar}
+  | .ldi .. =>
+    if m.psr.mode == .user && m.mar.isPrivilege then
+      .none
+    else
+      let aux : Address := Encodable.decode <| m.getMem m.mar
+      if m.psr.mode == .user && aux.isPrivilege then
+        .none
+      else
+        .some {m with mdr := m.getMem aux}
+  | _ => .some m
+
+/--
+The ***EXECUTE*** phase in the instruction cycle, where the instruction is actually executed.
+Except for *TRAP* and *RTI* instructions, in this phase, the instruction does not directly interact with the machine's main memory and uses `MAR` and `MDR` register instead.
+The data movement between those registers and the memory is carried out in ***FETCH OPERANDS*** and ***STORE RESULT*** phases: see `LC3.Machine.fetchOp` and `LC3.Machine.storeResult`.
+-/
+def execute (m : Machine) : Option Machine :=
+  match m.ir with
+  | .br n z p _ =>
+    if n && m.psr.n || z && m.psr.z || p && m.psr.p then
+      .some {m with pc := m.mar}
+    else
+      .some m
+  | .add dr sr1 rhs =>
+    let op2 := match rhs with | .reg i => m.getReg i | .imm n => n
+    let result := m.getReg sr1 + op2
+    let m := m.setReg dr result
+    .some <| m.setCC result
+  | .ld dr _ =>
+    let result := m.mdr
+    let m := m.setReg dr result
+    .some <| m.setCC result
+  | .st sr _ =>
+    .some {m with mdr := m.getReg sr}
+  | .jsr dr (.reg sr) =>
+    let aux : Int := Encodable.encode m.pc
+    let m := {m with
+      pc := Encodable.decode <| m.getReg sr
+    }
+    .some <| m.setReg dr aux
+  | .jsr dr (.imm _) =>
+    let m := m.setReg dr <| Encodable.encode m.pc
+    .some {m with pc := m.mar}
+  | .and dr sr1 rhs =>
+    let op2 := match rhs with | .reg i => m.getReg i | .imm n => n
+    let result := m.getReg sr1 &&& op2
+    let m := m.setReg dr result
+    .some <| m.setCC result
+  | .ldr dr _ _ =>
+    let result := m.mdr
+    let m := m.setReg dr result
+    .some <| m.setCC result
+  | .str sr _ _ =>
+    .some {m with mdr := m.getReg sr}
+  | .rti spr =>
+    if m.psr.mode = .user then
+      .none
+    else
+      let sp : Address := Encodable.decode <| m.getReg spr
+      let m := {m with
+        psr := Encodable.decode <| m.getMem (sp + (1 : Int))
+        pc := Encodable.decode <| m.getMem sp
+      }
+      let aux := sp + (2 : Int)
+      match m.psr.mode with
+      | .user =>
+        let m := m.setReg spr <| Encodable.encode m.sspr
+        .some <| {m with sspr := aux}
+      | .privilege =>
+        .some <| m.setReg spr <| Encodable.encode aux
+  | .xor dr sr1 rhs =>
+    let op2 := match rhs with | .reg i => m.getReg i | .imm n => n
+    let result := m.getReg sr1 ^^^ op2
+    let m := m.setReg dr result
+    .some <| m.setCC result
+  | .ldi dr _ =>
+    let result := m.mdr
+    let m := m.setReg dr result
+    .some <| m.setCC result
+  | .sti sr _ =>
+    .some {m with mdr := m.getReg sr}
+  | .jmp sr =>
+    .some {m with pc := Encodable.decode <| m.getReg sr}
+  | .reserved _ => m
+  | .lea dr _ =>
+    let result : Int := Encodable.encode m.mar
+    let m := m.setReg dr result
+    .some <| m.setCC result
+  | .trap .. =>
+    panic! "*TRAP* instruction has not been implemented yet."
+
+/--
+The ***STORE RESULT*** phase in the instruction cycle.
+It is only needed for *STORE XXX* instructions; i.e. *ST*, *STR*, *STI*.
+More precisely, the phase causes `mem[MAR] ← MDR` for *ST* and *STR* while `mem[mem[MAR]] ← MDR` for *STI*.
+The phase may give rise to the ACV exception if `m.psr.mode = .user` and if the memory location lies in the privileged range.
+-/
+def storeResult (m : Machine) : Option Machine :=
+  match m.ir with
+  | .st .. | .str .. =>
+    if m.psr.mode == .user && m.mar.isPrivilege then
+      .none
+    else
+      m.setMem m.mar m.mdr
+  | .sti .. =>
+    if m.psr.mode == .user && m.mar.isPrivilege then
+      .none
+    else
+      let aux : Address := Encodable.decode <| m.getMem m.mar
+      if m.psr.mode == .user && aux.isPrivilege then
+        .none
+      else
+        m.setMem aux m.mdr
+  | _ => m
+
+end Machine
+
+end LC3
